src/compiler/meta/OCL_compiler_parser_UML_extended.thy
@@ -45,7 +45,7 @@ header{* Part ... *}
 
 theory  OCL_compiler_parser_UML_extended
 imports OCL_compiler_meta_UML_extended
-        "../../compiler_generic/toy_example/embedding/meta_toy/Parser_oid"
+        "../../compiler_generic/meta_isabelle/Parser_init"
 begin
 
 section{* Generation to both Form (setup part) *}
@@ -80,6 +80,15 @@ subsubsection{* general *}
 
 context i_of
 begin
+
+definition "i_of_internal_oid a b = rec_internal_oid
+  (ap1 a (b \<open>Oid\<close>) (i_of_nat a b))"
+
+definition "i_of_internal_oids a b = rec_internal_oids
+  (ap3 a (b \<open>Oids\<close>)
+    (i_of_nat a b)
+    (i_of_nat a b)
+    (i_of_nat a b))"
 
 definition "i_of_ocl_def_base a b = rec_ocl_def_base
   (ap1 a (b \<open>OclDefInteger\<close>) (i_of_string a b))
@@ -133,6 +142,8 @@ definition "i_of_ocl_def_pre_post a b = rec_ocl_def_pre_post
 end
 
 lemmas [code] =
+  i_of.i_of_internal_oid_def
+  i_of.i_of_internal_oids_def
   i_of.i_of_ocl_def_base_def
   i_of.i_of_ocl_data_shallow_def
   i_of.i_of_ocl_list_attr_def
